examples/unit-tests/qs.fst
@@ -1,16 +1,14 @@
 module Quicksort
 open List
 
+(* Specification of sortedness according to some comparison function f *)
+val sorted: ('a -> Tot ('a -> Tot bool)) -> list 'a -> Tot bool
+let rec sorted f = function
+  | []
+  | [_] -> true
+  | x::y::tl -> f x y && sorted f (y::tl)
 
-val partition: f:('a -> Tot bool) -> list 'a -> Tot (list 'a * list 'a)
-let rec partition (a:Type) (f:a -> Tot bool) = function 
-  | [] -> [], []
-  | hd::tl -> 
-     let l1, l2 = partition f tl in
-     if f hd 
-     then hd::l1, l2
-     else l1, hd::l2
-
+(* A lemma about List.partition ... duh *)
 val partition_lemma: f:('a -> Tot bool)
                   -> l:list 'a
                   -> Lemma (requires True)
@@ -18,173 +16,46 @@ val partition_lemma: f:('a -> Tot bool)
                                      (length l1 + length l2 = length l
                                       /\ (forall x. mem x l1 ==> f x)
                                       /\ (forall x. mem x l2 ==> not (f x))
-                                      /\ (forall x. mem x l = mem x l1 || mem x l2)))
-                                    (fst (partition f l))
-                                    (snd (partition f l))))
-                           [SMTPat (partition f l)]
+                                      /\ (forall x. mem x l = (mem x l1 || mem x l2))))
+                                        (fst (partition f l))
+                                        (snd (partition f l))))
+                           [SMTPat (partition f l)] (* injected to the solver *)
 let rec partition_lemma f l = match l with 
   | [] -> ()
   | hd::tl -> partition_lemma f tl
 
-val quicksort: leq:('a -> Tot ('a -> Tot bool)) //Need to make the partial application explicit
-               -> l:list 'a
-               -> Tot (list 'a)
-                      (decreases (length l)) 
-let rec quicksort leq = function
-  | [] -> []
-  | pivot::tl ->
-     let hi, lo = partition (leq pivot) tl in
-     quicksort leq lo@[pivot]@quicksort leq hi
 
-logic type total_order (a:Type) (f: (a -> Tot (a -> Tot bool))) =
+opaque logic type total_order (a:Type) (f: (a -> Tot (a -> Tot bool))) =
     (forall a. f a a)                                           (* reflexivity   *)
-    /\ (forall a1 a2. f a1 a2 /\ (a1 <> a2) <==> not (f a2 a1)) (* anti-symmetry *)
+    /\ (forall a1 a2. (f a1 a2 /\ a1<>a2)  <==> not (f a2 a1))  (* anti-symmetry *)
     /\ (forall a1 a2 a3. f a1 a2 /\ f a2 a3 ==> f a1 a3)        (* transitivity  *)
 
-val sorted: ('a -> 'a -> Tot bool) -> list 'a -> Tot bool
-let rec sorted f = function
-  | []
-  | [_] -> true
-  | x::y::tl -> f x y && sorted f (y::tl)
-                                 
-
-val pivot_lemma: a:Type
-                 ->  f:(a -> Tot (a -> Tot bool))
-                 ->  l:list a
-                 ->  pivot:a
-                 ->  Lemma (requires (total_order a f))
-                           (ensures ((fun m1 m2 -> forall x y. mem x m1 /\ mem y m2 ==> f y x)
-                                       (fst (partition (f pivot) l))
-                                       (snd (partition (f pivot) l))))
-                           [SMTPat (partition (f pivot) l)]
-let rec pivot_lemma f l pivot = match l with
+val sorted_concat_lemma:  a:Type
+               ->  f:(a -> Tot (a -> Tot bool))
+               ->  l1:list a{sorted f l1}
+               ->  l2:list a{sorted f l2}
+               ->  pivot:a
+               ->  Lemma (requires (total_order a f
+                                    /\ (forall y. mem y l1 ==> not(f pivot y))
+                                    /\ (forall y. mem y l2 ==> f pivot y)))
+                         (ensures (sorted f (l1@(pivot::l2))))
+                         [SMTPat (sorted f (l1@(pivot::l2)))]
+let rec sorted_concat_lemma f l1 l2 pivot = match l1 with 
   | [] -> ()
-  | hd::tl -> pivot_lemma f tl pivot 
+  | hd::tl -> sorted_concat_lemma f tl l2 pivot
 
 
-val qs: a:Type
-            ->  f:(a -> Tot (a -> Tot bool))
-            ->  l:list a
-            ->  Lemma (requires (total_order a f))
-                      (ensures ((fun m -> sorted m /\ forall x. mem x l = mem x m)
-                                (quicksort f l)))
-let rec qs f l = match l with 
+(* The implemntation of quicksort: happily, the code is completely unpolluted by proof. *)
+val sort: f:('a -> Tot ('a -> Tot bool)) //Currying is explicit
+      ->  l:list 'a
+      ->  Pure (list 'a)
+               (requires (total_order 'a f))
+               (ensures (fun m -> sorted f m /\ (forall x. mem x l = mem x m)))
+               (decreases (length l))
+let rec sort f = function
   | [] -> []
   | pivot::tl -> 
-     let hi, lo = partition (f pivot) tl in 
-     lo@[pivot]@hi
-     
-
-
-
-
-
-(* (\* definining a non-strict total order *\) *)
-(* type NSTO (#'a:Type) ('R:'a => 'a => Type) =  *)
-(*     (forall (x:'a). 'R x x)                                    (\* reflexive *\) *)
-(*  /\ (forall (x:'a) (y:'a). 'R x y /\ x<>y  ==> not ('R y x))   (\* anti-symmetric *\) *)
-(*  /\ (forall (x:'a) (y:'a) (z:'a). 'R x y /\ 'R y z ==> 'R x z) (\* transitive *\) *)
-
-(* (\* sortedRange 'a 'R lo hi l : a list that has elements (x1 'R ... 'R xn) ... where a 'R x1 and xn 'R hi *\) *)
-(* logic val sortedRange: 'a:Type -> 'R:('a => 'a => Type) -> lo:'a -> hi:'a -> bool *)
-(* let rec sortedRange 'a ('R:'a => 'a => Type) lo hi = function *)
-(*   | [] -> as_bool ('R lo hi) *)
-(*   | hd::tl ->  as_bool ('R lo hd) && *)
-(*                as_bool ('R hd hi) && *)
-(*                sortedRange 'a 'R hd hi tl  *)
-      
-(* type nat = x:int{x>=0} *)
-
-(* val occurs : 'a --> list 'a --> nat *)
-(* let rec occurs x l : $decreases l = match l with *)
-(*   | [] -> 0 *)
-(*   | y::tl -> if x=y then 1 + occurs x tl else occurs x tl *)
-      
-(* type Permutation (#'a:Type) l m =  *)
-(*     forall x. occurs x l = occurs x m *)
-
-(* type Mem (#'a:Type) x l =  *)
-(*     occurs 'a x l > 0 *)
-
-(* type slist 'a 'R n1 n2 =  *)
-(*     i:list 'a{sortedRange 'a 'R n1 n2 i = true} *)
-
-(* val append: 'a:_ -> 'R:_ -> #n1:'a -> #n2:'a -> #n3:'a -> #n4:'a  *)
-(*          -> i:slist 'a 'R n1 n2 *)
-(*          -> j:slist 'a 'R n3 n4{'R n1 n2 /\ 'R n2 n3 /\ 'R n3 n4 /\ NSTO 'R} *)
-(*          -> k:slist 'a 'R n1 n4{forall x. occurs x k = occurs x i + occurs x j} *)
-(* let rec append 'a 'R n1 n2 n3 n4 i j = match i with  *)
-(*   | [] -> j *)
-(*   | hd::tl ->  *)
-(*     let tl : slist 'a 'R hd n2 = tl in  *)
-(*     hd::append tl j *)
-
-(* type decides ('a:Type) ('R:'a => 'a => Type) =  *)
-(*     cmp:(x:'a -> y:'a -> b:bool{(b=true <==> 'R x y) /\ (b=false <==> (x<>y /\ 'R y x))}){NSTO 'R} *)
-
-(* val partition: 'a:_ -> 'R:_  *)
-(*             -> cmp:decides 'a 'R *)
-(*             -> x:'a *)
-(*             -> l:list 'a *)
-(*             -> (lo:list 'a *)
-(*                 * hi:list 'a{(forall y. Mem y lo ==> 'R y x /\ Mem y l) *)
-(*                                /\ (forall y. Mem y hi ==> 'R x y /\ x<>y /\ Mem y l) *)
-(*                                /\ (forall y. occurs y l = occurs y lo + occurs y hi)}) *)
-(* let rec partition 'a 'R cmp x l = match l with *)
-(*   | [] -> ([], []) *)
-(*   | hd::tl -> *)
-(*     let lo, hi = partition 'a 'R cmp x tl in *)
-(*     if cmp hd x *)
-(*     then (hd::lo, hi) *)
-(*     else (lo, hd::hi) *)
-
-(* val quicksort: 'a:_ -> 'R:_ *)
-(*        -> cmp:decides 'a 'R *)
-(*        -> min:ghost 'a *)
-(*        -> max:ghost 'a{'R min max} *)
-(*        -> i:list 'a{forall x. Mem x i ==> ('R (unghost min) x /\ 'R x (unghost max))} *)
-(*        -> j:slist 'a 'r (unghost min) (unghost max){Permutation i j} *)
-(* let rec quicksort 'a 'R cmp min max i = match i with *)
-(*   | [] -> [] *)
-(*   | hd::tl -> *)
-(*     let lo, hi = partition cmp hd tl in *)
-(*     let i' = quicksort cmp min hd lo in *)
-(*     let j' = quicksort cmp hd max hi in *)
-(*     append i' (hd::j') *)
-
-(* (\*--------------------------------------------------------------------------------*\) *)
-(* (\* A client of quicksort for integers *\) *)
-(* (\*--------------------------------------------------------------------------------*\) *)
-(* let rec min = function  *)
-(*   | [] -> 0 *)
-(*   | [x] -> x *)
-(*   | hd::tl ->  *)
-(*     let x = min tl in *)
-(*     if leq x hd then x else hd *)
-
-(* let rec max = function  *)
-(*   | [] -> 0 *)
-(*   | [x] -> x *)
-(*   | hd::tl ->  *)
-(*     let x = max tl in *)
-(*     if x > hd then x else hd *)
-
-(* (\*  Would be nice to have such a syntax to introduce lemmas into the context *\) *)
-(* lemma val minmax : l:list 'a --> u:unit{min l <= max l} *)
-(* let rec minmax l : {decreases l} = match l with  *)
-(*   | [] -> () *)
-(*   | _::tl -> minmax tl *)
-
-(* lemma val minmem: x:'a --> l:list 'a{Mem x l} --> u:unit{min l <= x} *)
-(* let rec minmem x = function  (\* function is sugar for match+decreases *\) *)
-(*   | _::tl -> minmem x tl *)
-
-(* lemma val maxmem: x:'a --> l:list 'a{Mem x l} --> u:unit{x <= max l} *)
-(* let rec maxmem x = function *)
-(*   | _::tl -> maxmem x tl *)
- 
-(* type Sorted = fun m => exists a b. sortedRange int LTE a b m = true *)
-
-(* val sort_int : l:list int -> m:list int {Sorted m /\ Permutation l m} *)
-(* let sort_int l =  *)
-(*   quicksort int LTE (fun x y -> x <= y) (ghost (min l)) (ghost (max l)) l *)
+    let hi', lo' = partition (f pivot) tl in 
+    let lo = sort f lo' in
+    let hi = sort f hi' in
+    lo@(pivot::hi) 
